# Mathematics rules
### Sections
* [Binomial theorem](#binomial-theorem)
* [Sigma Notation](#sigma-notation)
* [Complex Numbers](#complex-numbers)
* [Propositional Logic](#propositional-logic)
___
### Notation
* <span style="color:red">def.</span> = definition

* <span style="color:purple">eg.</span> = example

* <span style="color:maroon">use.</span> = use case
___
## Binomial theorem

<span style="color:maroon">use.</span> to expand any binomial.

> $$
(a+b)^{n} =
\begin{pmatrix} n\\0 \end{pmatrix}
a^{n}b^{0} +
\begin{pmatrix} n\\1 \end{pmatrix}
a^{n-1}b^{1} +
\begin{pmatrix} n\\2 \end{pmatrix}
a^{n-2}b^{2} + ... +
\begin{pmatrix} n\\n \end{pmatrix}
a^{0}b^{n} 
$$

> $$
\begin{pmatrix} n\\k \end{pmatrix} = 
\frac{n!}{k!(n-k)!} = C_{k}^{n}
$$


<span style="color:purple">eg.</span> 
[One](./maths_e.md#binomial-theorem#example-1) 

The set of coefficients is symmetrical.

>$$
\begin{pmatrix} n\\k \end{pmatrix} =
\frac{n!}{k!(n-k)!}=
\frac{n!}{(n-k)!(n-(n-k))!}=
\begin{pmatrix} n\\n-k \end{pmatrix} 
$$

The 1st and last binomial coefficient are equel to 1 (as shown in the quote) and the

> $$
\begin{pmatrix} n\\0 \end{pmatrix} =
\begin{pmatrix} n\\n-0 \end{pmatrix} =
\frac{n!}{0!(n-0)!}=1
$$
___
## Sigma Notation
___
## Complex Numbers
___
## Propositional Logic

<span style="color:red">def.</span> Proposition: a statement that is either true or false.

<span style="color:purple">eg.</span> 
[One](./maths_e.md#propositional-logic) 
___